Progress on lock-free linear search.

mailbox/verif_lockfree_linsearch.v
@@ -37,12 +37,15 @@ Fixpoint index_of (m : list (Z * Z)) (k : Z) :=
                         else option_map Z.succ (index_of rest k)
   end.
 
-Lemma index_of_spec : forall k m, match index_of m k with Some i => 0 <= i /\ fst (Znth i m (0, 0)) = k
+Lemma index_of_spec : forall k m, match index_of m k with
+  | Some i => 0 <= i < Zlength m /\ fst (Znth i m (0, 0)) = k
   | None => ~In k (map fst m) end.
 Proof.
   induction m; simpl; auto; intros.
   destruct a.
-  destruct (eq_dec z k); [split; auto; computable|].
+  rewrite Zlength_cons.
+  pose proof (Zlength_nonneg m).
+  destruct (eq_dec z k); [split; auto; omega|].
   destruct (index_of m k); simpl.
   - destruct IHm; unfold Z.succ; rewrite Znth_pos_cons, Z.add_simpl_r; [split|]; auto; omega.
   - tauto.
@@ -66,8 +69,7 @@ Definition value_of e :=
 Definition last_value (h : hist) v :=
   (* initial condition *)
   (h = [] /\ v = vint 0) \/
-  exists n e, In (n, e) h /\ value_of e = v /\
-  Forall (fun x => let '(m, _) := x in m <= n)%nat h.
+  exists n e, In (n, e) h /\ value_of e = v /\ Forall (fun x => let '(m, _) := x in m <= n)%nat h.
 
 Lemma last_value_new : forall h n e, Forall (fun x => fst x < n)%nat h ->
   last_value (h ++ [(n, e)]) (value_of e).
@@ -79,20 +81,70 @@ Proof.
   destruct a; simpl in *; omega.
 Qed.
 
-Inductive compatible : list (hist * hist) -> list (Z * Z) -> Prop :=
-| compatible_nil : compatible [] []
-| compatible_cons k v m hk hv h (Hk : last_value hk (vint k)) (Hv : last_value hv (vint v)) :
-    compatible ((hk, hv) :: h) ((k, v) :: m)
-| compatible_zero hk hv h (Hzero : last_value hk (vint 0)) :
-    compatible ((hk, hv) :: h) [].
+Definition compatible h m := Forall2 (fun hs e => last_value (fst hs) (vint (fst e)) /\
+  last_value (snd hs) (vint (snd e))) (sublist 0 (Zlength m) h) m /\
+  Forall (fun hs => last_value (fst hs) (vint 0)) (sublist (Zlength m) (Zlength h) h).
 
-Definition wf_map (m : list (Z * Z)) := ~In 0 (map fst m).
+Definition ordered_hist h := forall i j (Hi : 0 <= i < j) (Hj : j < Zlength h),
+  (fst (Znth i h (O, Store (vint 0))) < fst (Znth j h (O, Store (vint 0))))%nat.
+
+Lemma ordered_cons : forall t e h, ordered_hist ((t, e) :: h) ->
+  Forall (fun x => let '(m, _) := x in t < m)%nat h /\ ordered_hist h.
+Proof.
+  unfold ordered_hist; split.
+  - rewrite Forall_forall; intros (?, ?) Hin.
+    apply In_Znth with (d := (O, Store (vint 0))) in Hin.
+    destruct Hin as (j & ? & Hj).
+    exploit (H 0 (j + 1)); try omega.
+    { rewrite Zlength_cons; omega. }
+    rewrite Znth_0_cons, Znth_pos_cons, Z.add_simpl_r, Hj by omega; auto.
+  - intros; exploit (H (i + 1) (j + 1)); try omega.
+    { rewrite Zlength_cons; omega. }
+    rewrite !Znth_pos_cons, !Z.add_simpl_r by omega; auto.
+Qed.
+
+Lemma ordered_last : forall t e h (Hordered : ordered_hist h) (Hin : In (t, e) h)
+  (Ht : Forall (fun x => let '(m, _) := x in m <= t)%nat h), last h (O, Store (vint 0)) = (t, e).
+Proof.
+  induction h; [contradiction | simpl; intros].
+  destruct a; apply ordered_cons in Hordered; destruct Hordered as (Ha & ?).
+  inversion Ht as [|??? Hp]; subst.
+  destruct Hin as [Hin | Hin]; [inv Hin|].
+  - destruct h; auto.
+    inv Ha; inv Hp; destruct p; omega.
+  - rewrite IHh; auto.
+    destruct h; auto; contradiction.
+Qed.
+
+Lemma ordered_last_value : forall h v (Hordered : ordered_hist h),
+  last_value h v <-> value_of (snd (last h (O, Store (vint 0)))) = v.
+Proof.
+  unfold last_value; split; intro.
+  - destruct H as [(? & ?) | (? & ? & ? & ? & ?)]; subst; auto.
+    erewrite ordered_last; eauto; auto.
+  - destruct h; [auto | right].
+    destruct (last (p :: h) (O, Store (vint 0))) as (t, e) eqn: Hlast.
+    exploit (@app_removelast_last _ (p :: h)); [discriminate | intro Heq].
+    rewrite Hlast in Heq.
+    exists t; exists e; repeat split; auto.
+    + rewrite Heq, in_app; simpl; auto.
+    + unfold ordered_hist in Hordered.
+      rewrite Forall_forall; intros (?, ?) Hin.
+      apply In_Znth with (d := (O, Store (vint 0))) in Hin.
+      destruct Hin as (i & ? & Hi).
+      rewrite <- Znth_last in Hlast.
+      destruct (eq_dec i (Zlength (p :: h) - 1)).
+      * subst; rewrite Hlast in Hi; inv Hi; auto.
+      * exploit (Hordered i (Zlength (p :: h) - 1)); try omega.
+        rewrite Hlast, Hi; simpl; omega.
+Qed.
+
+Definition wf_map (m : list (Z * Z)) := Forall (fun i => repable_signed i /\ i <> 0) (map fst m).
 
 Definition int_op e :=
   match e with
-  | Load v => exists i, v = Vint i
-  | Store v => exists i, v = Vint i
-  | CAS r c w => exists i1 i2 i3, r = Vint i1 /\ c = Vint i2 /\ w = Vint i3
+  | Load v | Store v => tc_val tint v
+  | CAS r c w => tc_val tint r /\ tc_val tint c /\ tc_val tint w
   end.
 
 (* Once set, a key is never reset. *)
@@ -118,6 +170,9 @@ Definition set_item_trace (h : list (hist * hist)) k v i h' :=
       Znth i h' ([], []) = (hk ++ [(t, CAS r (vint 0) (vint k))], hv ++ [(tv, Store (vint v))]) /\
       (r = vint 0 \/ r = vint k)) /\ sublist (i + 1) (Zlength h) h = sublist (i + 1) (Zlength h') h'.
 
+Definition int_hists (h : list (hist * hist)) := Forall (fun x => Forall int_op (map snd (fst x)) /\
+                                                 Forall int_op (map snd (snd x))) h.
+
 (* What can a thread know?
    At least certain keys exist, and whatever it did last took effect.
    It can even rely on the indices of known keys. *)
@@ -126,6 +181,7 @@ Definition set_item_spec :=
   WITH key : Z, value : Z, p : val, sh : share, entries : list val, h : list (hist * hist), m : list (Z * Z)
   PRE [ _key OF tint, _value OF tint ]
    PROP (repable_signed key; repable_signed value; readable_share sh; Forall isptr entries; Zlength h = 20;
+         Forall (fun x => ordered_hist (fst x) /\ ordered_hist (snd x)) h; int_hists h;
          wf_map m; compatible h m)
    LOCAL (temp _key (vint key); temp _value (vint value); gvar _m_entries p)
    SEP (data_at sh (tarray (tptr tentry) 20) entries p;
@@ -133,7 +189,9 @@ Definition set_item_spec :=
         entry_hists entries h)
   POST [ tvoid ]
    EX i : Z, EX h' : list (hist * hist), EX m' : list (Z * Z),
-   PROP (set_item_trace h key value i h'; wf_map m'; compatible (sublist 0 i h') m';
+   PROP (Forall (fun x => ordered_hist (fst x) /\ ordered_hist (snd x)) h'; int_hists h';
+         set_item_trace h key value i h';
+         wf_map m'; compatible (sublist 0 i h' ++ sublist i (Zlength h) h) m';
          compatible h' (set m' key value); incl m m')
    LOCAL ()
    SEP (data_at sh (tarray (tptr tentry) 20) entries p;
@@ -153,17 +211,22 @@ Definition get_item_trace (h : list (hist * hist)) k v h' := exists i,
 (* Read the most recently written value. *)
 Definition get_item_spec :=
  DECLARE _get_item
-  WITH key : Z, p : val, sh : share, entries : list val, h : list (hist * hist)
+  WITH key : Z, p : val, sh : share, entries : list val, h : list (hist * hist), m : list (Z * Z)
   PRE [ _key OF tint, _value OF tint ]
-   PROP (repable_signed key; readable_share sh; Forall isptr entries; Zlength h = 20)
+   PROP (repable_signed key; readable_share sh; Forall isptr entries; Zlength h = 20;
+         Forall (fun x => ordered_hist (fst x) /\ ordered_hist (snd x)) h; int_hists h;
+         wf_map m; compatible h m)
    LOCAL (temp _key (vint key); gvar _m_entries p)
    SEP (data_at sh (tarray (tptr tentry) 20) entries p;
         fold_right_sepcon (map (atomic_entry sh) entries);
         entry_hists entries h)
   POST [ tint ]
-   EX value : Z, EX h' : list (hist * hist),
-   PROP (get_item_trace h key value h')
-   LOCAL ()
+   EX value : Z, EX h' : list (hist * hist), EX m' : list (Z * Z),
+   PROP (Forall (fun x => ordered_hist (fst x) /\ ordered_hist (snd x)) h'; int_hists h';
+         wf_map m'; compatible h' m'; get_item_trace h key value h';
+         if eq_dec value 0 then ~In key (map fst m') /\ incl m m'
+         else get m' key = Some value /\ incl (set m key value) m')
+   LOCAL (temp ret_temp (vint value))
    SEP (data_at sh (tarray (tptr tentry) 20) entries p;
         fold_right_sepcon (map (atomic_entry sh) entries);
         entry_hists entries h').
@@ -198,20 +261,221 @@ Ltac entailer_for_return ::= go_lower; entailer'.
 
 Definition make_int v := match v with Vint i => Int.signed i | _ => 0 end.
 
+Lemma apply_int_ops : forall v h i (Hv : verif_atomics.apply_hist (Vint i) h = Some v)
+  (Hints : Forall int_op h), tc_val tint v.
+Proof.
+  induction h; simpl; intros.
+  - inv Hv; eauto.
+  - inversion Hints as [|?? Ha]; subst.
+    destruct a.
+    + destruct (eq_dec v0 (Vint i)); [eapply IHh; eauto | discriminate].
+    + destruct v0; try contradiction; eapply IHh; eauto.
+    + destruct (eq_dec r (Vint i)); [|discriminate].
+      destruct Ha as (? & ? & ?).
+      destruct w; try contradiction.
+      destruct (eq_dec c (Vint i)); eapply IHh; eauto.
+Qed.
+
+Lemma compatible_length : forall h m, compatible h m -> Zlength m <= Zlength h.
+Proof.
+  intros ?? (? & ?).
+  apply mem_lemmas.Forall2_Zlength in H.
+  pose proof (sublist_max_length 0 (Zlength m) h); omega.
+Qed.
+
+Lemma compatible_app : forall h1 h2 m1 m2 (Hcompat1 : compatible h1 m1) (Hcompat2 : compatible h2 m2),
+  Zlength h1 = Zlength m1 -> compatible (h1 ++ h2) (m1 ++ m2).
+Proof.
+  intros; pose proof (compatible_length _ _ Hcompat2).
+  destruct Hcompat1 as (Hh1 & _), Hcompat2 as (Hh2 & Hrest); unfold compatible.
+  rewrite !Zlength_app.
+  pose proof (Zlength_nonneg m1); pose proof (Zlength_nonneg m2).
+  rewrite !sublist_app by omega.
+  rewrite H, !Z.add_simpl_l.
+  rewrite Z.min_l, Z.min_r, Z.max_r, Z.max_l by omega.
+  rewrite Z.min_r, Z.max_l by omega.
+  rewrite sublist_nil, sublist_same; auto; simpl; split; auto.
+  rewrite sublist_same in Hh1; auto.
+  apply Forall2_app; auto.
+Qed.
+
+Lemma ordered_snoc : forall h t e, ordered_hist h -> Forall (fun x => fst x < t)%nat h ->
+  ordered_hist (h ++ [(t, e)]).
+Proof.
+  repeat intro.
+  rewrite Zlength_app, Zlength_cons, Zlength_nil in Hj.
+  rewrite app_Znth1 by omega.
+  destruct (eq_dec j (Zlength h)).
+  - rewrite Znth_app1; auto.
+    apply Forall_Znth; auto; omega.
+  - specialize (H i j).
+    rewrite app_Znth1 by omega; apply H; auto; omega.
+Qed.
+
+Lemma compatible_sublist : forall h m i j, compatible h m -> 0 <= i -> j <= Zlength m ->
+  compatible (sublist i j h) (sublist i j m).
+Proof.
+  intros; unfold compatible.
+  pose proof (compatible_length _ _ H).
+  destruct (Z_le_dec j i).
+  { rewrite sublist_nil_gen with (l0 := m); auto.
+    rewrite sublist_nil_gen with (l0 := h); auto.
+    rewrite sublist_nil; split; auto; constructor. }
+  rewrite Zlength_sublist, sublist_sublist by omega.
+  rewrite Zlength_sublist, sublist_sublist by omega.
+  rewrite sublist_nil; split; auto.
+  destruct H.
+  rewrite Z.add_0_l, Z.sub_simpl_r.
+  replace (sublist i j h) with (sublist i j (sublist 0 (Zlength m) h)).
+  apply Forall2_sublist; auto.
+  { rewrite sublist_sublist by omega; f_equal; omega. }
+Qed.
+
+Lemma failed_CAS_fst : forall v h h', Forall2 (failed_CAS v) h h' -> map snd h' = map snd h.
+Proof.
+  induction 1; auto.
+  destruct H as (? & ? & ? & ? & ? & ?); simpl; f_equal; auto.
+Qed.
+
+Lemma make_int_spec : forall v, tc_val tint v -> vint (make_int v) = v.
+Proof.
+  destruct v; try contradiction; simpl.
+  rewrite Int.repr_signed; auto.
+Qed.
+
+Definition make_map h := (map (fun x => (make_int (value_of (snd (last (fst x) (O, Store (vint 0))))),
+  make_int (value_of (snd (last (snd x) (O, Store (vint 0))))))) h).
+
+Lemma compatible_nil : compatible [] [].
+Proof.
+  split; rewrite sublist_of_nil; auto.
+Qed.
+Hint Resolve compatible_nil.
+
+Lemma compatible_cons : forall a b h m
+  (Hkey : last_value (fst a) (vint (fst b))) (Hvalue : last_value (snd a) (vint (snd b)))
+  (Hrest : compatible h m), compatible (a :: h) (b :: m).
+Proof.
+  unfold compatible; intros.
+  pose proof (Zlength_nonneg m).
+  rewrite !Zlength_cons, sublist_0_cons, sublist_S_cons by omega.
+  unfold Z.succ; rewrite !Z.add_simpl_r.
+  destruct Hrest; split; auto.
+Qed.
+
+Lemma int_op_value : forall e, int_op e -> tc_val tint (value_of e).
+Proof.
+  destruct e; auto; simpl.
+  intros (? & ? & ?); destruct (eq_dec r c); auto.
+Qed.
+
+Lemma make_compatible : forall h
+  (Hordered : Forall (fun x => ordered_hist (fst x) /\ ordered_hist (snd x)) h) (Hint : int_hists h),
+  Forall2 (fun hs e => last_value (fst hs) (vint (fst e)) /\ last_value (snd hs) (vint (snd e)))
+    h (make_map h).
+Proof.
+  induction 1; intro; [constructor | simpl].
+  inversion Hint as [|?? (Hfst & Hsnd)]; subst; destruct H.
+  rewrite Forall_map in Hfst, Hsnd.
+  exploit (Forall_last _ (O, Store (vint 0)) _ Hfst); simpl; auto.
+  exploit (Forall_last _ (O, Store (vint 0)) _ Hsnd); simpl; auto.
+  intro Hfst'; apply int_op_value in Hfst'.
+  intro Hsnd'; apply int_op_value in Hsnd'.
+  constructor; auto.
+  rewrite !ordered_last_value; auto; simpl; rewrite !make_int_spec; auto.
+Qed.
+
+Lemma compatible_set : forall h m hk hv i k v (Hcompat : compatible h m)
+  (Hcase : index_of m k = Some i \/ index_of m k = None /\ i = Zlength m) (Hi : i < Zlength h)
+  (Hkey : last_value hk (vint k)) (Hvalue : last_value hv (vint v)),
+  compatible (upd_Znth i h (hk, hv)) (set m k v).
+Proof.
+  intros.
+  pose proof (index_of_spec k m) as Hk.
+  pose proof (compatible_length _ _ Hcompat).
+  unfold compatible.
+  destruct Hcase as [Hcase | (Hcase & ?)]; subst.
+  - unfold set; rewrite Hcase in *; destruct Hk.
+    rewrite !upd_Znth_Zlength by (auto; omega).
+    rewrite sublist_upd_Znth_r with (lo := Zlength m) by omega.
+    destruct Hcompat; split; auto.
+    rewrite sublist_upd_Znth_lr, Z.sub_0_r by omega.
+    apply Forall2_upd_Znth; auto.
+    rewrite Zlength_sublist; omega.
+  - unfold set; rewrite Hcase in *.
+    pose proof (Zlength_nonneg m).
+    rewrite !upd_Znth_Zlength by auto.
+    rewrite Zlength_app, Zlength_cons, Zlength_nil; simpl.
+    rewrite sublist_upd_Znth_r with (lo := Zlength m + 1) by omega.
+    destruct Hcompat as (? & Hzero); split.
+    + rewrite sublist_upd_Znth_lr, Z.sub_0_r by omega.
+      rewrite sublist_split with (mid := Zlength m) by omega.
+      assert (Zlength (sublist 0 (Zlength m) h) = Zlength m) as Hlen.
+      { rewrite Zlength_sublist; auto; omega. }
+      rewrite upd_Znth_app2, Hlen, Zminus_diag.
+      apply Forall2_app; auto.
+      erewrite sublist_len_1 with (d := ([] : hist, [] : hist)) by auto.
+      rewrite upd_Znth0, sublist_nil; constructor; auto.
+      { rewrite Hlen; split; [omega|].
+        rewrite <- Z.le_sub_le_add_l, Zminus_diag; apply Zlength_nonneg. }
+    + rewrite sublist_next with (d := ([] : hist, [] : hist)) in Hzero by (auto; omega).
+      inv Hzero; auto.
+Qed.
+
+Lemma index_of_app : forall k m1 m2, index_of (m1 ++ m2) k =
+  match index_of m1 k with Some i => Some i | None => option_map (Z.add (Zlength m1)) (index_of m2 k) end.
+Proof.
+  induction m1; simpl; intros.
+  - destruct (index_of m2 k); auto.
+  - destruct a.
+    destruct (eq_dec z k); auto.
+    rewrite IHm1; destruct (index_of m1 k); auto; simpl.
+    destruct (index_of m2 k); auto; simpl.
+    rewrite Zlength_cons; f_equal; omega.
+Qed.
+
+Lemma index_of_out : forall k m, Forall (fun x => fst x <> k) m -> index_of m k = None.
+Proof.
+  intros.
+  pose proof (index_of_spec k m) as Hk.
+  destruct (index_of m k); auto.
+  destruct Hk; rewrite Forall_forall in H; exploit (H (Znth z m (0, 0))); auto; try contradiction.
+  apply Znth_In; auto.
+Qed.
+
 Lemma body_set_item : semax_body Vprog Gprog f_set_item set_item_spec.
 Proof.
   start_function.
   forward.
   eapply semax_pre with (P' := EX i : Z, EX h' : list (hist * hist),
-    PROP (0 <= i < 20; Forall2 (failed_CAS key) (sublist 0 i h) (sublist 0 i h');
-          (* Not just that it's a failed CAS, but that it reads the corresponding value in m. *)
+    PROP (0 <= i < 20; Forall (fun x => ordered_hist (fst x) /\ ordered_hist (snd x)) h'; int_hists h';
+          Forall2 (failed_CAS key) (sublist 0 i h) (sublist 0 i h');
+          Forall2 (fun hs e => last_value (fst hs) (vint (fst e)) /\ last_value (snd hs) (vint (snd e)))
+            (sublist 0 (Zlength m) h') m;
           sublist i (Zlength h) h = sublist i (Zlength h') h')
     LOCAL (temp _idx (vint i); temp _key (vint key); temp _value (vint value); gvar _m_entries p)
     SEP (data_at sh (tarray (tptr tentry) 20) entries p; fold_right_sepcon (map (atomic_entry sh) entries);
          entry_hists entries h')).
-  { Exists 0 h; rewrite sublist_nil; entailer!. }
+  { Exists 0 h; rewrite sublist_nil; entailer!.
+    match goal with H : compatible h m |- _ => destruct H; auto end. }
   eapply semax_loop.
   - Intros i h'; forward.
+    assert (Zlength h' = Zlength h) as Hlen.
+    { assert (Zlength (sublist i (Zlength h) h) = Zlength (sublist i (Zlength h') h')) as Heq
+        by (replace (sublist i (Zlength h) h) with (sublist i (Zlength h') h'); auto).
+      rewrite !Zlength_sublist in Heq; try omega.
+      destruct (Z_le_dec i (Zlength h')); [omega|].
+      unfold sublist in Heq.
+      rewrite Z2Nat_neg in Heq by omega.
+      simpl in Heq; rewrite Zlength_nil in Heq; omega. }
+    assert (i <= Zlength h') by omega.
+    assert (map snd h' = map snd h) as Hsnd.
+    { erewrite <- sublist_same with (al := h') by eauto.
+      erewrite <- sublist_same with (al := h) by eauto.
+      rewrite sublist_split with (al := h')(mid := i) by omega.
+      rewrite sublist_split with (al := h)(mid := i) by omega.
+      rewrite Hlen in *; rewrite !map_app; f_equal; [|congruence].
+      eapply failed_CAS_fst; eauto. }
     assert_PROP (Zlength entries = 20) by entailer!.
     assert (0 <= i < Zlength entries) by (replace (Zlength entries) with 20; auto).
     forward.
@@ -224,42 +488,27 @@ Proof.
     rewrite atomic_loc_isptr.
     forward.
     forward.
+    destruct (Znth i h' ([], [])) as (hki, hvi) eqn: Hhi.
     forward_call (Tsh, sh, field_address tentry [StructField _key] (Znth i entries Vundef), lkey, vint 0,
-      vint key, vint 0, fst (Znth i h' ([], [])),
-      fun (h : hist) c v => !!(c = vint 0 /\ v = vint key /\ h = fst (Znth i h' ([], []))) && emp,
+      vint key, vint 0, hki,
+      fun (h : hist) c v => !!(c = vint 0 /\ v = vint key /\ h = hki) && emp,
       k_R,
-      fun (h : hist) (v : val) => !!(forall v0, last_value (fst (Znth i h' ([], []))) v0 -> v0 <> vint 0 ->
-        v = v0) && emp).
+      fun (h : hist) (v : val) => !!(forall v0, last_value hki v0 -> v0 <> vint 0 -> v = v0) && emp).
 (* Given that I have to do this, maybe better to remove the arguments from P. *)
     { entailer!.
       rewrite field_address_offset; simpl.
       rewrite isptr_offset_val_zero; auto.
       { rewrite field_compatible_cons; simpl.
         split; [unfold in_members; simpl|]; auto. } }
+    { replace hki with (fst (Znth i h' ([], []))) by (rewrite Hhi; auto); fast_cancel. }
     { repeat (split; auto).
       intros ?????????????? Ha.
       unfold k_R in *; simpl in *.
       eapply semax_pre, Ha.
       go_lowerx; entailer!.
-Lemma apply_int_ops : forall v h i (Hv : verif_atomics.apply_hist (Vint i) h = Some v) (Hints : Forall int_op h),
-  exists i', v = Vint i'.
-Proof.
-  induction h; simpl; intros.
-  - inv Hv; eauto.
-  - inversion Hints as [|?? Ha]; subst.
-    destruct a.
-    + destruct (eq_dec v0 (Vint i)); [eauto | discriminate].
-    + destruct Ha; subst; eauto.
-    + destruct (eq_dec r (Vint i)); [|discriminate].
-      destruct Ha as (? & i' & ? & ? & ? & ?); subst.
-      destruct (eq_dec (Vint i') (Vint i)); eauto.
-Qed.
-
       repeat split.
       + rewrite Forall_app; repeat constructor; auto.
         apply apply_int_ops in Hvx; auto.
-        destruct Hvx; subst.
-        simpl; repeat eexists.
       + intros ? Hin; rewrite in_app in Hin.
         destruct Hin as [? | [? | ?]]; [| |contradiction].
         * intros.
@@ -284,29 +533,24 @@ Qed.
       destruct (eq_dec i0 (Int.repr key)).
       + subst; rewrite Int.eq_true; apply drop_tc_environ.
       + rewrite Int.eq_false; [apply drop_tc_environ | auto]. }
-    assert (Zlength h' = Zlength h).
-    { assert (Zlength (sublist i (Zlength h) h) = Zlength (sublist i (Zlength h') h')) as Heq
-        by (replace (sublist i (Zlength h) h) with (sublist i (Zlength h') h'); auto).
-      rewrite !Zlength_sublist in Heq; try omega.
-      destruct (Z_le_dec i (Zlength h')); [omega|].
-      unfold sublist in Heq.
-      rewrite Z2Nat_neg in Heq by omega.
-      simpl in Heq; rewrite Zlength_nil in Heq; omega. }
-    match goal with H : sublist _ _ h = sublist _ _ h' |- _ =>
-      erewrite sublist_next with (d := ([] : hist, [] : hist)),
-               sublist_next with (l := h')(d := ([] : hist, [] : hist)) in H by omega; inversion H as [Heq] end.
+    assert (Znth i h ([], []) = Znth i h' ([], []) /\
+      sublist (i + 1) (Zlength h) h = sublist (i + 1) (Zlength h') h') as (Heq & Hi1).
+    { match goal with H : sublist _ _ h = sublist _ _ h' |- _ =>
+        erewrite sublist_next with (d := ([] : hist, [] : hist)),
+                 sublist_next with (l := h')(d := ([] : hist, [] : hist)) in H by omega; inv H; auto end. }
     match goal with |- semax _ (PROP () (LOCALx ?Q (SEPx ?R))) _ _ =>
       forward_if (PROP (i0 <> Int.zero /\ i0 <> Int.repr key) (LOCALx Q (SEPx R))) end.
     + rewrite (atomic_loc_isptr _ lval).
       forward.
       forward.
       forward_call (Tsh, sh, field_address tentry [StructField _value] (Znth i entries Vundef), lval,
-        vint value, vint 0, snd (Znth i h' ([], [])), fun (h : hist) v => !!(v = vint value) && emp,
+        vint value, vint 0, hvi, fun (h : hist) v => !!(v = vint value) && emp,
         v_R, fun (h : hist) => emp).
       { entailer!.
         rewrite field_address_offset; auto.
         { rewrite field_compatible_cons; simpl.
           split; [unfold in_members; simpl|]; auto. } }
+      { replace hvi with (snd (Znth i h' ([], []))) by (rewrite Hhi; auto); fast_cancel. }
       { repeat (split; auto).
         intros ????????????? Ha.
         unfold v_R in *; simpl in *.
@@ -317,85 +561,211 @@ Qed.
       Intros t'.
       forward.
       Exists i (upd_Znth i h' (fst (Znth i h' ([], [])) ++ [(t, CAS (Vint i0) (vint 0) (vint key))],
-        snd (Znth i h' ([], [])) ++ [(t', Store (vint value))]))
-        (m ++ map (fun x => (make_int (value_of (snd (last (fst x) (O, Store (vint 0))))), 0))
-                  (sublist (Zlength m) i h')).
+        snd (Znth i h' ([], [])) ++ [(t', Store (vint value))])) (m ++ make_map (sublist (Zlength m) i h')).
       apply andp_right; auto.
       apply andp_right.
-      { apply prop_right; repeat split.
-        - rewrite sublist_upd_Znth_l; auto; omega.
-        - rewrite upd_Znth_same by omega.
-          replace (Znth i h ([], [])) with (Znth i h' ([], [])).
-          destruct (Znth i h' ([], [])).
-          repeat eexists; eauto.
-          destruct (eq_dec i0 Int.zero); subst; auto.
-          destruct (eq_dec i0 (Int.repr key)); subst; auto.
-          absurd (Int.zero = Int.zero); auto.
-        - rewrite upd_Znth_Zlength by omega.
-          rewrite sublist_upd_Znth_r; auto; omega.
+      { assert (0 <= i < Zlength h') by (rewrite Hlen; omega).
+        assert (Zlength m <= Zlength h').
+        { rewrite Hlen; apply compatible_length; auto. }
+        assert (compatible (sublist 0 i h' ++ sublist i (Zlength h) h)
+                           (m ++ make_map (sublist (Zlength m) i h'))).
+        { destruct (Z_lt_dec i (Zlength m)).
+          + rewrite (sublist_nil_gen _ (Zlength m)), app_nil_r by omega.
+            replace (sublist i (Zlength h) h) with (sublist i (Zlength h') h').
+            rewrite sublist_rejoin, sublist_same by omega.
+            split; auto.
+            replace (sublist (Zlength m) (Zlength h') h') with (sublist (Zlength m) (Zlength h) h).
+            match goal with H : compatible h m |- _ => destruct H; auto end.
+            transitivity (sublist (Zlength m - i) (Zlength h - i) (sublist i (Zlength h) h)).
+            * rewrite sublist_sublist, !Z.sub_simpl_r by omega; auto.
+            * replace (sublist i (Zlength h) h) with (sublist i (Zlength h') h').
+              rewrite Hlen, sublist_sublist, !Z.sub_simpl_r by omega; auto.
+          + pose proof (Zlength_nonneg m).
+            rewrite sublist_split with (mid := (Zlength m)) by omega.
+            rewrite <- app_assoc; apply compatible_app.
+            * assert (Zlength (sublist 0 (Zlength m) h') = Zlength m).
+              { rewrite Zlength_sublist; omega. }
+              unfold compatible; rewrite sublist_same; auto.
+              split; auto.
+              rewrite sublist_nil'; auto.
+            * pose proof (Zlength_nonneg (sublist (Zlength m) i h')).
+              pose proof (Zlength_nonneg (sublist i (Zlength h) h)).
+              split.
+              unfold make_map at 1; rewrite Zlength_map, sublist_app.
+              rewrite Z.min_l by auto.
+              rewrite Z.min_l, sublist_same by (auto; apply Z.le_refl).
+              rewrite Zminus_diag.
+              rewrite !Z.max_r, sublist_nil, app_nil_r by (auto; omega).
+              apply make_compatible.
+              { apply Forall_sublist; auto. }
+              { apply Forall_sublist; auto. }
+              { split; auto; apply Z.le_refl. }
+              { rewrite <- Z.le_sub_le_add_l, Zminus_diag; auto. }
+              { unfold make_map; rewrite Zlength_map, Zlength_app.
+                rewrite sublist_app; try omega.
+                rewrite Z.min_r, Z.min_r, sublist_nil; try (apply Z.le_refl); try omega.
+                rewrite Zminus_diag, Z.max_l, Z.add_simpl_l, Z.max_l, sublist_same; try (apply Z.le_refl);
+                  auto.
+                match goal with H : compatible h m |- _ => destruct H as (_ & Hzero) end.
+                apply Forall_sublist with (lo := i - Zlength m)(hi := Zlength h - Zlength m) in Hzero.
+                rewrite sublist_sublist, !Z.sub_simpl_r in Hzero by omega; auto.
+                { split; auto.
+                  rewrite <- Z.le_sub_le_add_l, Zminus_diag; auto. } }
+            * rewrite Zlength_sublist; auto; omega. }
+        apply prop_right; split; [|split; [|split; [|split; [|split; [|split]]]]].
+        - apply Forall_upd_Znth; auto; rewrite Hhi; simpl.
+          exploit (Znth_In i h' ([], [])); [auto | rewrite Hhi; intro Hin].
+          match goal with H : Forall _ h' |- _ => rewrite Forall_forall in H; specialize (H _ Hin);
+            destruct H end.
+          split; apply ordered_snoc; auto.
+        - apply Forall_upd_Znth; auto.
+          match goal with H : int_hists h' |- _ => unfold int_hists in H; rewrite Forall_forall in H;
+            exploit (H (Znth i h' ([], []))) end.
+          { apply Znth_In; auto. }
+          intros (? & ?); simpl.
+          rewrite !map_app, !Forall_app; repeat split; auto; constructor; simpl; eauto 6.
+        - split; [rewrite sublist_upd_Znth_l; auto; omega|].
+          split.
+          + rewrite upd_Znth_same by omega.
+            replace (Znth i h ([], [])) with (Znth i h' ([], [])).
+            destruct (Znth i h' ([], [])).
+            repeat eexists; eauto.
+            destruct (eq_dec i0 Int.zero); subst; auto.
+            destruct (eq_dec i0 (Int.repr key)); subst; auto.
+            absurd (Int.zero = Int.zero); auto.
+          + rewrite upd_Znth_Zlength by omega.
+            rewrite sublist_upd_Znth_r; auto; omega.
         - unfold wf_map in *.
-          intro Hin; rewrite map_app, in_app in Hin; destruct Hin as [? | Hin]; [absurd (In 0 (map fst m)); auto|].
-          rewrite in_map_iff in Hin; destruct Hin as (? & Hzero & Hin).
-          rewrite in_map_iff in Hin; destruct Hin as (? & ? & Hin); subst; simpl in *.
-
-Lemma Forall2_In_r : forall A B (P : A -> B -> Prop) x l1 l2, Forall2 P l1 l2 -> In x l2 ->
-  exists y, In y l1 /\ P y x.
-Proof.
-  induction 1; intro Hin; destruct Hin; simpl.
-  - subst; eauto.
-  - destruct IHForall2 as (? & ? & ?); eauto.
-Qed.
-
-Lemma last_snoc : forall A (d : A) x l, last (l ++ [x]) d = x.
-Proof.
-  induction l; auto; simpl.
-  destruct (l ++ [x]) eqn: Heq; auto.
-  contradiction (app_cons_not_nil l [] x); auto.
-Qed.
+          rewrite map_app, Forall_app; split; auto.
+          unfold make_map; rewrite !Forall_map.
+          rewrite Forall_forall; intros ? Hin; simpl.
+          apply In_Znth with (d := ([], [])) in Hin.
+          destruct Hin as (j & Hj & Hjth).
           destruct (Z_le_dec i (Zlength m)).
-          { rewrite sublist_nil_gen in Hin; auto. }
-          exploit Forall2_In_r; eauto.
-          { eapply sublist_In.
-            rewrite sublist_sublist, 2Z.add_0_r; eauto; try omega.
-            split; [apply Zlength_nonneg | omega]. }
-          intros (? & ? & ? & v & Hfst & ? & ? & ?).
-          setoid_rewrite Hfst in Hzero.
-          rewrite last_snoc in Hzero; simpl in Hzero.
-          destruct (eq_dec (Vint v) (vint 0)); [absurd (v = Int.zero); auto; inv e; auto|].
-          simpl in Hzero.
-          absurd (v = Int.zero); auto.
-(* up *)
-Lemma signed_inj : forall i1 i2, Int.signed i1 = Int.signed i2 -> i1 = i2.
-Proof.
-  intros.
-  apply int_eq_e.
-  rewrite Int.eq_signed, H.
-  apply zeq_true.
-Qed.
+          { rewrite sublist_nil_gen, Zlength_nil in Hj; omega. }
+          match goal with H : Forall2 (failed_CAS key) _ _ |- _ => exploit (Forall2_In_r _ x _ _ H) end.
+          { exploit (Znth_In j (sublist (Zlength m) i h') ([], [])); auto; intro.
+            eapply sublist_In; rewrite sublist_sublist, 2Z.add_0_r; subst; eauto; try omega.
+            pose (Zlength_nonneg m); omega. }
+          intros (? & ? & ? & r & Heqi & ? & ? & ?); subst.
+          setoid_rewrite Heqi; rewrite last_snoc; simpl.
+          destruct (eq_dec (Vint r) (vint 0)).
+          { absurd (r = Int.zero); auto; inv e; auto. }
+          simpl.
+          split; [apply Int.signed_range|].
+          intro; absurd (r = Int.zero); auto.
           apply signed_inj; auto.
-        - rewrite sublist_upd_Znth_l by omega.
-          rewrite sublist_split with (mid := Zlength m); try omega.
-
-Lemma compatible_app : forall h1 h2 m1 m2, compatible h1 m1 -> compatible h2 m2 -> Zlength h1 = Zlength m1 ->
-  compatible (h1 ++ h2) (m1 ++ m2).
-Proof.
-  induction 1; auto; simpl; intros.
-  - constructor; auto.
-  - rewrite Zlength_cons, Zlength_nil in *.
-    pose proof (Zlength_nonneg h); omega.
-Qed.
-          apply compatible_app.
-          + 
-
-
-          + admit.
-          + rewrite Zlength_sublist; try omega.
-            admit.
-            admit.
-          + admit.
-          + admit.
-        - admit.
-        - apply incl_appl, incl_refl. }
+        - rewrite sublist_upd_Znth_l by omega; auto.
+        - match goal with H : Forall (fun x => ordered_hist (fst x) /\ ordered_hist (snd x)) h' |- _ =>
+            rewrite Forall_forall in H; exploit (H (Znth i h' ([], []))) end.
+          { apply Znth_In; auto. }
+          rewrite Hhi; intros (? & ?).
+          apply compatible_set;
+            try (rewrite ordered_last_value, last_snoc; simpl; auto; try (apply ordered_snoc; auto)).
+          + match goal with H : compatible _ _ |- _ => replace (sublist i (Zlength h) h) with
+              (sublist i (Zlength h') h') in H; rewrite sublist_rejoin, sublist_same in H; auto; omega end.
+          + assert (Forall (fun x => fst x <> key) (sublist 0 i (m ++ make_map (sublist (Zlength m) i h'))))
+              as Hmiss.
+            { rewrite Forall_forall; intros ? Hin.
+              rewrite sublist_app, in_app in Hin; try omega.
+              assert (exists hk hv, In (hk, hv) (sublist 0 i h') /\
+                value_of (snd (last hk (O, Store (vint 0)))) = vint (fst x)) as (hk & hv & Hin' & Hlast).
+              { destruct Hin as [Hin | Hin].
+                * pose proof (Zlength_nonneg m); rewrite Z.min_l in Hin by auto.
+                  apply In_Znth with (d := (0, 0)) in Hin.
+                  destruct Hin as (j & (? & Hj) & Hx).
+                  rewrite Zlength_sublist in Hj.
+                  rewrite Znth_sublist in Hx by (auto; omega).
+                  rewrite Z.sub_0_r, Z.min_glb_lt_iff in Hj; destruct Hj.
+                  match goal with H : Forall2 _ (sublist _ _ _) m |- _ =>
+                    exploit (Forall2_Znth _ _ _ ([] : hist, [] : hist) (0, 0) H j) end.
+                  { rewrite Zlength_sublist; auto; omega. }
+                  rewrite Z.add_0_r in Hx; rewrite Hx.
+                  replace (Znth j (sublist 0 (Zlength m) h') ([] : hist, [] : hist)) with
+                    (Znth j (sublist 0 i h') ([], [])).
+                  destruct (Znth j (sublist 0 i h') ([], [])) eqn: Hj.
+                  simpl; intros (? & _).
+                  do 3 eexists.
+                  { rewrite <- Hj; apply Znth_In.
+                    rewrite Zlength_sublist; auto; omega. }
+                  rewrite <- ordered_last_value; auto.
+                  match goal with H : forall x, In x h' -> ordered_hist (fst x) /\ _ |- _ =>
+                    exploit (H (Znth j (sublist 0 i h') ([], []))) end.
+                  { rewrite Znth_sublist by omega; apply Znth_In.
+                    match goal with H : compatible h m |- _ => apply compatible_length in H end.
+                    setoid_rewrite Hlen; omega. }
+                  rewrite Hj; simpl; tauto.
+                  { rewrite !Znth_sublist; auto; omega. }
+                  { split; [apply Z.le_refl|].
+                    apply Z.min_glb; auto; omega. }
+                  { apply Z.le_min_r. }
+                * apply sublist_In in Hin.
+                  unfold make_map in Hin; rewrite in_map_iff in Hin.
+                  destruct Hin as ((?, ?) & ? & Hin); subst; simpl.
+                  destruct (Z_le_dec i (Zlength m)).
+                  { rewrite sublist_nil_gen in Hin; auto; contradiction. }
+                  do 3 eexists.
+                  { pose proof (Zlength_nonneg m).
+                    rewrite sublist_split with (mid := (Zlength m)) by omega.
+                    rewrite in_app; eauto. }
+                  symmetry; apply make_int_spec, int_op_value, Forall_last; auto.
+                  match goal with H : int_hists h' |- _ => unfold int_hists in H; rewrite Forall_forall in H;
+                    exploit (H (l, l0)) end.
+                  { eapply sublist_In; eauto. }
+                  rewrite Forall_map; tauto. }
+              match goal with H : Forall2 (failed_CAS key) _ _ |- _ =>
+                exploit (Forall2_In_r _ (hk, hv) _ _ H); auto end.
+              intros (? & ? & ? & r & Heqi & ? & ? & ?); subst.
+              simpl in Heqi; rewrite Heqi, last_snoc in Hlast; simpl in Hlast.
+              destruct (eq_dec (Vint r) (vint 0)).
+              { absurd (r = Int.zero); auto; inv e; auto. }
+              inversion Hlast.
+              intro; absurd (r = Int.repr key); subst; auto.
+              { unfold make_map; rewrite Zlength_map.
+                destruct (Z_le_dec i (Zlength m)).
+                { rewrite sublist_nil_gen, Zlength_nil, Z.add_0_r; auto. }
+                pose proof (Zlength_nonneg m).
+                rewrite Zlength_sublist; auto; omega. } }
+            destruct (Z_lt_dec i (Zlength m)).
+            * left; rewrite sublist_nil_gen, app_nil_r by (auto; omega).
+              rewrite sublist_nil_gen with (i1 := Zlength m), app_nil_r in Hmiss by omega.
+              replace m with (sublist 0 i m ++ Znth i m (0, 0) :: sublist (i + 1) (Zlength m) m).
+              rewrite index_of_app, index_of_out; auto; simpl.
+              destruct (Znth i m (0, 0)) eqn: Hi.
+              assert (z = key).
+              { match goal with H : Forall2 _ (sublist _ _ _) m |- _ =>
+                  exploit (Forall2_Znth _ _ _ ([] : hist, [] : hist) (0, 0) H i) end.
+                { rewrite Zlength_sublist; auto; omega. }
+                rewrite Znth_sublist, Z.add_0_r, Hi by omega.
+                setoid_rewrite Hhi; intros (Hkey & _).
+                match goal with H : wf_map m |- _ => unfold wf_map in H; rewrite Forall_forall in H;
+                  exploit (H z) end.
+                { rewrite in_map_iff; exists (z, z0); split; auto.
+                  rewrite <- Hi; apply Znth_In; omega. }
+                intros (? & ?).
+                assert (repable_signed 0) by (split; computable).
+                match goal with H : forall v0, last_value hki v0 -> v0 <> vint 0 -> Vint i0 = v0 |- _ =>
+                  exploit H; eauto end.
+                { intro; absurd (z = 0); auto; apply repr_inj_signed; auto.
+                  simpl in *; congruence. }
+                intro X; inv X.
+                destruct (eq_dec (Int.repr z) Int.zero); [absurd (z = 0); auto; apply repr_inj_signed; auto|].
+                destruct (eq_dec (Int.repr z) (Int.repr key)); [|absurd (Int.repr 0 = Int.zero); auto].
+                apply repr_inj_signed; auto. }
+              subst; rewrite eq_dec_refl; simpl.
+              rewrite Zlength_sublist by omega; f_equal; omega.
+              { rewrite <- sublist_next, sublist_rejoin, sublist_same; auto; omega. }
+            * right; pose proof (Zlength_nonneg m).
+              assert (i = Zlength (m ++ make_map (sublist (Zlength m) i h'))).
+              { unfold make_map; rewrite Zlength_app, Zlength_map, Zlength_sublist; auto; omega. }
+              split; auto.
+              rewrite sublist_same in Hmiss; auto.
+              apply index_of_out; auto.
+          + omega.
+          + destruct (eq_dec i0 Int.zero); subst; auto.
+            destruct (eq_dec i0 (Int.repr key)); [|absurd (Int.repr 0 = Int.zero); auto].
+            subst; if_tac; auto.
+        - split; auto; apply incl_appl, incl_refl. }
       apply andp_right; auto.
       fast_cancel.
       rewrite (sepcon_comm (ghost_hist _ _)).
@@ -418,7 +788,7 @@ Qed.
         destruct (eq_dec i1 i).
         subst; rewrite upd_Znth_same by (rewrite Zlength_map; auto).
         erewrite Znth_map, Znth_upto; simpl; auto; try omega.
-        rewrite upd_Znth_same; auto; simpl.
+        rewrite upd_Znth_same, Hhi; auto; simpl.
         { rewrite upd_Znth_diff; auto.
           rewrite Zlength_upto in *.
           erewrite !Znth_map, !Znth_upto; auto; try omega.
@@ -433,7 +803,10 @@ Qed.
       destruct (eq_dec ek EK_normal); [subst | apply drop_tc_environ].
       Intros; unfold POSTCONDITION, abbreviate, normal_ret_assert, loop1_ret_assert.
       instantiate (1 := EX i : Z, EX h' : list (hist * hist),
-        PROP (0 <= i < 20; Forall2 (failed_CAS key) (sublist 0 (i + 1) h) (sublist 0 (i + 1) h');
+        PROP (0 <= i < 20; Forall (fun x => ordered_hist (fst x) /\ ordered_hist (snd x)) h'; int_hists h';
+              Forall2 (failed_CAS key) (sublist 0 (i + 1) h) (sublist 0 (i + 1) h');
+              Forall2 (fun hs e => last_value (fst hs) (vint (fst e)) /\ last_value (snd hs) (vint (snd e)))
+                (sublist 0 (Zlength m) h') m;
               sublist (i + 1) (Zlength h) h = sublist (i + 1) (Zlength h') h')
         LOCAL (temp _idx (vint i); temp _key (vint key); temp _value (vint value); gvar _m_entries p)
         SEP (data_at sh (tarray (tptr tentry) 20) entries p; fold_right_sepcon (map (atomic_entry sh) entries);
@@ -442,7 +815,20 @@ Qed.
         snd (Znth i h' ([], [])))).
       go_lower.
       apply andp_right.
-      { apply prop_right; repeat (split; auto).
+      { assert (0 <= i < Zlength h') by (rewrite Hlen; omega).
+        match goal with H : Forall _ h' |- _ => rewrite Forall_forall in H;
+          exploit (H (Znth i h' ([], []))); rewrite <- Forall_forall in H end.
+        { apply Znth_In; auto. }
+        intros (? & ?).
+        apply prop_right; repeat (split; auto).
+        * apply Forall_upd_Znth; auto; simpl.
+          split; auto; apply ordered_snoc; auto; rewrite Hhi; auto.
+        * apply Forall_upd_Znth; auto; simpl.
+          match goal with H : int_hists h' |- _ => unfold int_hists in H; rewrite Forall_forall in H;
+            exploit (H (Znth i h' ([], []))) end.
+          { apply Znth_In; auto. }
+          intros (? & ?); split; auto.
+          rewrite map_app, Forall_app; split; auto; repeat constructor.
         * erewrite sublist_split, sublist_len_1 with (i1 := i); try omega.
           erewrite sublist_split with (hi := i + 1), sublist_len_1 with (i1 := i)(d := ([] : hist, [] : hist));
             rewrite ?upd_Znth_Zlength; try omega.
@@ -452,6 +838,34 @@ Qed.
           constructor; auto.
           unfold failed_CAS; simpl.
           rewrite Heq; repeat eexists; eauto.
+        * destruct (Z_le_dec (Zlength m) i).
+          { pose proof (Zlength_nonneg m); rewrite sublist_upd_Znth_l by omega; auto. }
+          rewrite sublist_upd_Znth_lr; try omega.
+          eapply Forall2_upd_Znth_l; auto; try omega; simpl.
+          match goal with H : compatible h m |- _ => pose proof (compatible_length _ _ H);
+            destruct H as (Hcompat & _) end.
+          exploit (Forall2_Znth _ _ _ ([] : hist, [] : hist) (0, 0) Hcompat i).
+          { rewrite Zlength_sublist; auto; omega. }
+          rewrite !Znth_sublist, Z.add_0_r, Z.sub_0_r by omega.
+          setoid_rewrite Heq.
+          intros (? & ?); split; eauto.
+          evar (R : val); replace (vint (fst (Znth i m (0, 0)))) with R; subst R;
+            [apply last_value_new; rewrite Hhi; auto | simpl].
+          destruct (eq_dec (Vint i0) (vint 0)).
+          { absurd (i0 = Int.zero); auto; inv e; auto. }
+          rewrite Hhi in *; simpl in *.
+          match goal with H : forall v0, _ -> _ -> Vint i0 = v0 |- _ => apply H; auto end.
+          match goal with H : wf_map m |- _ => unfold wf_map in H; rewrite Forall_map, Forall_forall in H;
+            exploit (H (Znth i m (0, 0))) end.
+          { apply Znth_In; omega. }
+          simpl; intros (? & ?).
+          intro X; absurd (fst (Znth i m (0, 0)) = 0); auto; apply repr_inj_signed; auto.
+          { split; computable. }
+          { congruence. }
+          { rewrite Zlength_sublist; try omega.
+            rewrite Hlen; apply compatible_length; auto. }
+          { rewrite Hlen; split; [omega|].
+            apply compatible_length; auto. }
         * rewrite upd_Znth_Zlength by omega.
           rewrite sublist_upd_Znth_r by omega; auto. }
       apply andp_right; [apply prop_right; auto|].
@@ -476,12 +890,13 @@ Qed.
         subst; rewrite upd_Znth_same by (rewrite Zlength_map; auto).
         erewrite Znth_map, Znth_upto; simpl; auto; try omega.
         rewrite upd_Znth_same; auto; simpl.
+        setoid_rewrite Hhi.
         rewrite sepcon_comm; auto.
         { rewrite upd_Znth_diff; auto.
           rewrite Zlength_upto in *.
           erewrite !Znth_map, !Znth_upto; auto; try omega.
           rewrite upd_Znth_diff; auto.
-          match goal with H : Zlength h' = _ |- _ => setoid_rewrite H; simpl in *; omega end. }
+          setoid_rewrite Hlen; simpl in *; omega. }
   - Intros i h'.
     forward.
     unfold loop2_ret_assert.
@@ -489,17 +904,27 @@ Qed.
     admit. (* list is long enough *)
 Admitted.
 
+Lemma failed_load_fst : forall v h h', Forall2 (failed_load v) h h' -> map snd h' = map snd h.
+Proof.
+  induction 1; auto.
+  destruct H as (? & ? & ? & ? & ? & ?); simpl; f_equal; auto.
+Qed.
+
 Lemma body_get_item : semax_body Vprog Gprog f_get_item get_item_spec.
 Proof.
   start_function.
   forward.
   eapply semax_pre with (P' := EX i : Z, EX h' : list (hist * hist),
-    PROP (0 <= i < 20; Forall2 (failed_load key) (sublist 0 i h) (sublist 0 i h');
+    PROP (0 <= i < 20; Forall (fun x => ordered_hist (fst x) /\ ordered_hist (snd x)) h'; int_hists h';
+          Forall2 (failed_load key) (sublist 0 i h) (sublist 0 i h');
+          Forall2 (fun hs e => last_value (fst hs) (vint (fst e)) /\ last_value (snd hs) (vint (snd e)))
+            (sublist 0 (Zlength m) h') m;
           sublist i (Zlength h) h = sublist i (Zlength h') h')
     LOCAL (temp _idx (vint i); temp _key (vint key); gvar _m_entries p)
     SEP (data_at sh (tarray (tptr tentry) 20) entries p; fold_right_sepcon (map (atomic_entry sh) entries);
          entry_hists entries h')).
-  { Exists 0 h; rewrite sublist_nil; entailer!. }
+  { Exists 0 h; rewrite sublist_nil; entailer!.
+    match goal with H : compatible h m |- _ => destruct H; auto end. }
   eapply semax_loop.
   - Intros i h'; forward.
     assert_PROP (Zlength entries = 20) by entailer!.
@@ -514,23 +939,7 @@ Proof.
     rewrite atomic_loc_isptr.
     forward.
     forward.
-    forward_call (Tsh, sh, field_address tentry [StructField _key] (Znth i entries Vundef), lkey, vint 0,
-      fst (Znth i h' ([], [])), fun (h : hist) => emp, e_R, fun (h : hist) (v : val) => emp).
-    { entailer!.
-      rewrite field_address_offset; simpl.
-      rewrite isptr_offset_val_zero; auto.
-      { rewrite field_compatible_cons; simpl.
-        split; [unfold in_members; simpl|]; auto. } }
-    { repeat (split; auto).
-      intros ???????????? Ha.
-      unfold e_R in *; simpl in *.
-      eapply semax_pre, Ha.
-      go_lowerx; entailer!.
-      apply andp_right; auto.
-      eapply derives_trans, precise_weak_precise; auto. }
-    Intros x; destruct x as (t, v); simpl in *.
-    destruct v; try contradiction.
-    assert (Zlength h' = Zlength h).
+    assert (Zlength h' = Zlength h) as Hlen.
     { assert (Zlength (sublist i (Zlength h) h) = Zlength (sublist i (Zlength h') h')) as Heq
         by (replace (sublist i (Zlength h) h) with (sublist i (Zlength h') h'); auto).
       rewrite !Zlength_sublist in Heq; try omega.
@@ -538,23 +947,63 @@ Proof.
       unfold sublist in Heq.
       rewrite Z2Nat_neg in Heq by omega.
       simpl in Heq; rewrite Zlength_nil in Heq; omega. }
-    match goal with H : sublist _ _ h = sublist _ _ h' |- _ =>
-      erewrite sublist_next with (d := ([] : hist, [] : hist)),
-               sublist_next with (l := h')(d := ([] : hist, [] : hist)) in H by omega; inversion H as [Heq] end.
+    assert (i < Zlength h') by omega.
+    assert (map snd h' = map snd h) as Hsnd.
+    { erewrite <- sublist_same with (al := h') by eauto.
+      erewrite <- sublist_same with (al := h) by eauto.
+      rewrite sublist_split with (al := h')(mid := i) by omega.
+      rewrite sublist_split with (al := h)(mid := i) by omega.
+      rewrite Hlen in *; rewrite !map_app; f_equal; [|congruence].
+      eapply failed_load_fst; eauto. }
+    destruct (Znth i h' ([], [])) as (hki, hvi) eqn: Hhi.
+    forward_call (Tsh, sh, field_address tentry [StructField _key] (Znth i entries Vundef), lkey, vint 0,
+      hki, fun h => !!(h = hki) && emp, k_R,
+      fun (h : hist) (v : val) => !!(forall v0, last_value hki v0 -> v0 <> vint 0 -> v = v0) && emp).
+    { entailer!.
+      rewrite field_address_offset; simpl.
+      rewrite isptr_offset_val_zero; auto.
+      { rewrite field_compatible_cons; simpl.
+        split; [unfold in_members; simpl|]; auto. } }
+    { replace hki with (fst (Znth i h' ([], []))) by (rewrite Hhi; auto); fast_cancel. }
+    { repeat (split; auto).
+      intros ???????????? Ha.
+      unfold k_R in *; simpl in *.
+      eapply semax_pre, Ha.
+      go_lowerx; entailer!.
+      repeat split.
+      + rewrite Forall_app; repeat constructor; auto.
+        apply apply_int_ops in Hvx; auto.
+      + intros ? Hin; rewrite in_app in Hin.
+        destruct Hin as [? | [? | ?]]; subst; auto; contradiction.
+      + intros ? [(? & ?) | (? & ? & Hin & ? & ?)] Hn; [contradiction Hn; auto|].
+        specialize (Hhist _ _ Hin); apply nth_error_In in Hhist; subst; auto.
+      + apply andp_right; auto.
+        eapply derives_trans, precise_weak_precise, precise_andp2; auto. }
+    Intros x; destruct x as (t, v); simpl in *.
+    destruct v; try contradiction.
+    assert (Zlength h' = Zlength h).
+    { assert (Zlength (sublist i (Zlength h) h) = Zlength (sublist i (Zlength h') h')) as Heq
+        by (replace (sublist i (Zlength h) h) with (sublist i (Zlength h') h'); auto).
+      rewrite !Zlength_sublist in Heq; omega. }
+    assert (Znth i h ([], []) = Znth i h' ([], []) /\
+      sublist (i + 1) (Zlength h) h = sublist (i + 1) (Zlength h') h') as (Heq & Hi1).
+    { match goal with H : sublist _ _ h = sublist _ _ h' |- _ =>
+        erewrite sublist_next with (d := ([] : hist, [] : hist)),
+                 sublist_next with (l := h')(d := ([] : hist, [] : hist)) in H by omega; inv H; auto end. }
     match goal with |- semax _ (PROP () (LOCALx ?Q (SEPx ?R))) _ _ =>
       forward_if (PROP (i0 <> Int.repr key) (LOCALx Q (SEPx R))) end.
     + rewrite (atomic_loc_isptr _ lval).
       forward.
       forward.
       forward_call (Tsh, sh, field_address tentry [StructField _value] (Znth i entries Vundef), lval, vint 0,
-        snd (Znth i h' ([], [])), fun (h : hist) => emp, e_R, fun (h : hist) (v : val) => emp).
+        snd (Znth i h' ([], [])), fun (h : hist) => emp, v_R, fun (h : hist) (v : val) => emp).
       { entailer!.
         rewrite field_address_offset; auto.
         { rewrite field_compatible_cons; simpl.
           split; [unfold in_members; simpl|]; auto. } }
       { repeat (split; auto).
         intros ???????????? Ha.
-        unfold e_R in *; simpl in *.
+        unfold v_R in *; simpl in *.
         eapply semax_pre, Ha.
         go_lowerx; entailer!.
         apply andp_right; auto.
@@ -562,10 +1011,43 @@ Proof.
       Intros x; destruct x as (t', v); simpl in *.
       forward.
       Exists (Int.signed v) (upd_Znth i h' (fst (Znth i h' ([], [])) ++ [(t, Load (vint key))],
-        snd (Znth i h' ([], [])) ++ [(t', Load (Vint v))])).
+        snd (Znth i h' ([], [])) ++ [(t', Load (Vint v))])) (m ++ make_map (sublist (Zlength m) i h')).
       apply andp_right.
-      { apply prop_right.
-        unfold get_item_trace.
+      { assert (In (Znth i h' ([], [])) h').
+        { apply Znth_In; split; auto; omega. }
+        match goal with H : Forall _ h' |- _ => rewrite Forall_forall in H;
+          exploit (H (Znth i h' ([], []))); auto; rewrite <- Forall_forall in H end.
+        intros (? & ?).
+        apply prop_right; split; [|split; [|split; [|split; [|split; [|split]]]]].
+        - apply Forall_upd_Znth; auto.
+          split; apply ordered_snoc; auto.
+          rewrite Hhi; auto.
+        - apply Forall_upd_Znth; auto; simpl.
+          match goal with H : int_hists h' |- _ => unfold int_hists in H; rewrite Forall_forall in H;
+            exploit (H (Znth i h' ([], []))); auto end.
+          intros (? & ?); rewrite !map_app, !Forall_app; repeat split; auto; repeat constructor.
+        - unfold wf_map; rewrite map_app, Forall_app; split; auto.
+(* Clean up some of this redundancy. *)
+          unfold make_map; rewrite !Forall_map.
+          rewrite Forall_forall; intros ? Hin; simpl.
+          apply In_Znth with (d := ([], [])) in Hin.
+          destruct Hin as (j & Hj & Hjth).
+          destruct (Z_le_dec i (Zlength m)).
+          { rewrite sublist_nil_gen, Zlength_nil in Hj; omega. }
+          match goal with H : Forall2 (failed_CAS key) _ _ |- _ => exploit (Forall2_In_r _ x _ _ H) end.
+          { exploit (Znth_In j (sublist (Zlength m) i h') ([], [])); auto; intro.
+            eapply sublist_In; rewrite sublist_sublist, 2Z.add_0_r; subst; eauto; try omega.
+            pose (Zlength_nonneg m); omega. }
+          intros (? & ? & ? & r & Heqi & ? & ? & ?); subst.
+          setoid_rewrite Heqi; rewrite last_snoc; simpl.
+          destruct (eq_dec (Vint r) (vint 0)).
+          { absurd (r = Int.zero); auto; inv e; auto. }
+          simpl.
+          split; [apply Int.signed_range|].
+          intro; absurd (r = Int.zero); auto.
+          apply signed_inj; auto.
+        - 
+
         split; auto.
         exists i; split; [|split].
         * rewrite sublist_upd_Znth_l; auto; omega.
